Taskin/DFA_rlin2.thy
@@ -1,7 +1,12 @@
 theory DFA_rlin2
 imports
-  Right_Linear "$AFP/Regular-Sets/Regular_Set"
+  Right_Linear
 begin
+
+text
+\<open>We define \<open>nxts_rlin2_set P M w\<close> that traverses the terminals list \<open>w\<close> starting from the set of non-terminals \<open>M\<close> according to
+ the production set \<open>P\<close>. At the end it gives the reachable non-terminals set. The definition is very similar to a 
+ nondeterministic finite automata\<close>
 
 definition nxt_rlin2 :: "('n,'t)Prods \<Rightarrow> 'n \<Rightarrow> 't \<Rightarrow> 'n set" where
 "nxt_rlin2 P A a = {B. (A, [Tm a, Nt B]) \<in> P}"
@@ -11,6 +16,8 @@ definition nxt_rlin2_set :: "('n,'t)Prods \<Rightarrow> 'n set \<Rightarrow> 't 
 
 definition nxts_rlin2_set :: "('n,'t)Prods \<Rightarrow> 'n set \<Rightarrow> 't list \<Rightarrow> 'n set" where
 "nxts_rlin2_set P = foldl (nxt_rlin2_set P)"
+
+subsection \<open>Properties of \<open>nxts_rlin2_set\<close>\<close>
 
 lemma nxt_rlin2_nts:
   assumes "B\<in>nxt_rlin2 P A a"
@@ -99,20 +106,6 @@ lemma nxts_trans2:
     shows "B \<in> nxts_rlin2_set P {A} (x@z)"
   using assms nxts_trans1[of "{C}" P A x B z] by auto
 
-lemma map_Tm_single_nt:
-  assumes "map Tm w @ [Tm a, Nt A] = u1 @ [Nt B] @ u2"
-  shows "u1 = map Tm (w @ [a]) \<and> u2 = []"
-proof -
-  from assms have *: "map Tm (w @ [a]) @ [Nt A] = u1 @ [Nt B] @ u2" by simp
-  have 1: "Nt B \<notin> set (map Tm (w @ [a]))" by auto
-  have 2: "Nt B \<in> set (u1 @ [Nt B] @ u2)" by simp
-  from * 1 2 have "Nt B \<in> set ([Nt A])"
-    by (metis list.set_intros(1) rotate1.simps(2) set_ConsD set_rotate1 sym.inject(1))
-  hence "[Nt B] = [Nt A]" by simp
-  with 1 * show ?thesis
-    by (metis append_Cons append_Cons_eq_iff append_self_conv emptyE empty_set)
-qed
-
 lemma nxts_to_mult_derive:
   "B \<in> nxts_rlin2_set P M w \<Longrightarrow> (\<exists>A\<in>M. P \<turnstile> [Nt A] \<Rightarrow>* map Tm w @ [Nt B])"
 unfolding nxts_rlin2_set_def proof (induction w arbitrary: B rule: rev_induct)
@@ -136,101 +129,6 @@ next
   with A_in show ?case by blast
 qed
 
-lemma rlin2_derive:
-  assumes "P \<turnstile> v1 \<Rightarrow>* v2" 
-      and "v1 = [Nt A]"
-      and "v2 = u1 @ [Nt B] @ u2" 
-      and "rlin2 P"
-    shows "\<exists>w. u1 = map Tm w \<and> u2 = []"
-using assms proof (induction arbitrary: u1 B u2 rule: rtrancl_derive_induct)
-  case base
-  then show ?case
-    by (simp add: append_eq_Cons_conv)
-next
-  case (step u C v w)
-  from step.prems(1) step.prems(3) have "\<exists>w. u = map Tm w \<and> v = []" 
-    using step.IH[of u C v] by simp
-  then obtain wh where u_def: "u = map Tm wh" by blast
-  have v_eps: "v = []"
-    using \<open>\<exists>w. u = map Tm w \<and> v = []\<close> by simp
-  from step.hyps(2) step.prems(3) have w_cases: "w = [] \<or> (\<exists>d D. w = [Tm d, Nt D])"
-    unfolding rlin2_def by auto
-  then show ?case proof cases
-    assume "w=[]"
-    with v_eps step.prems(2) have "u = u1 @ [Nt B] @ u2" by simp
-    with u_def show ?thesis by simp (metis ex_map_conv in_set_conv_decomp sym.distinct(1))
-  next
-    assume "\<not>w=[]"
-    then obtain d D where "w = [Tm d, Nt D]" 
-      using w_cases by blast
-    with u_def v_eps step.prems(2) have "u1 = map Tm (wh @ [d]) \<and> u2 = []"
-      using map_Tm_single_nt[of wh d D u1 B u2] by simp
-    thus ?thesis by blast
-  qed
-qed
-
-lemma rlin2_introduce_tm:
-  assumes "rlin2 P"
-      and "P \<turnstile> [Nt A] \<Rightarrow>* map Tm w @ [Tm x, Nt B]"
-    shows "\<exists>C. P \<turnstile> [Nt A] \<Rightarrow>* map Tm w @ [Nt C] \<and> (C,[Tm x, Nt B]) \<in> P"
-proof -
-  from assms(2) have "\<exists>v. P \<turnstile> [Nt A] \<Rightarrow>* v \<and> P \<turnstile> v \<Rightarrow> map Tm w @ [Tm x, Nt B]"
-    using rtranclp.cases by fastforce
-  then obtain v where v_star: "P \<turnstile> [Nt A] \<Rightarrow>* v" and v_step: "P \<turnstile> v \<Rightarrow> map Tm w @ [Tm x, Nt B]" by blast
-  from v_step have "\<exists>u1 u2 C \<alpha>. v = u1 @ [Nt C] @ u2 \<and> map Tm w @ [Tm x, Nt B] = u1 @ \<alpha> @ u2 \<and> (C,\<alpha>) \<in> P"
-    using derive.cases by fastforce
-  then obtain u1 u2 C \<alpha> where v_def: "v = u1 @ [Nt C] @ u2" and w_def: "map Tm w @ [Tm x, Nt B] = u1 @ \<alpha> @ u2" 
-                          and C_prod: "(C,\<alpha>) \<in> P" by blast
-  from assms(1) v_star v_def have u2_eps: "u2 = []"
-    using rlin2_derive[of P "[Nt A]"] by simp
-  from assms(1) v_star v_def obtain wa where u1_def: "u1 = map Tm wa"
-    using rlin2_derive[of P "[Nt A]" "u1 @ [Nt C] @ u2" A u1] by auto
-  from w_def u2_eps u1_def have "map Tm w @ [Tm x, Nt B] = map Tm wa @ \<alpha>" by simp
-  then have "map Tm (w @ [x]) @ [Nt B] = map Tm wa @ \<alpha>" by simp
-  then have "\<alpha> \<noteq> []" 
-    by (metis append.assoc append.right_neutral list.distinct(1) map_Tm_single_nt)
-  with assms(1) C_prod obtain d D where "\<alpha> = [Tm d, Nt D]"
-    using rlin2_def by fastforce
-  from w_def u2_eps have x_d: "x = d" 
-    using \<open>\<alpha> = [Tm d, Nt D]\<close> by simp
-  from w_def u2_eps have B_D: "B = D"
-    using \<open>\<alpha> = [Tm d, Nt D]\<close> by simp
-  from x_d B_D have alpha_def: "\<alpha> = [Tm x, Nt B]"
-    using \<open>\<alpha> = [Tm d, Nt D]\<close> by simp
-  from w_def u2_eps alpha_def have "map Tm w = u1" by simp
-  with u1_def have w_eq_wa: "w = wa"
-    by (metis list.inj_map_strong sym.inject(2))
-  from v_def u1_def w_eq_wa u2_eps have "v = map Tm w @ [Nt C]" by simp
-  with v_star have 1: "P \<turnstile> [Nt A] \<Rightarrow>* map Tm w @ [Nt C]" by simp
-  from C_prod alpha_def have 2: "(C,[Tm x, Nt B]) \<in> P" by simp
-  from 1 2 show ?thesis by auto
-qed
-
-lemma rlin2_nts_derive_eq: 
-  assumes "rlin2 P"
-      and "P \<turnstile> [Nt A] \<Rightarrow>* [Nt B]"
-    shows "A = B"
-proof -
-  from assms(2) have star_cases: "[Nt A] = [Nt B] \<or> (\<exists>w. P \<turnstile> [Nt A] \<Rightarrow> w \<and> P \<turnstile> w \<Rightarrow>* [Nt B])"
-    using converse_rtranclpE by force
-  show ?thesis proof cases
-    assume "\<not>[Nt A] = [Nt B]"
-    then obtain w where w_step: "P \<turnstile> [Nt A] \<Rightarrow> w" and w_star: "P \<turnstile> w \<Rightarrow>* [Nt B]"
-      using star_cases by auto
-    from assms(1) w_step have w_cases: "w = [] \<or> (\<exists>a C. w = [Tm a, Nt C])"
-      unfolding rlin2_def using derive_singleton[of P "Nt A" w] by auto
-    show ?thesis proof cases
-      assume "w = []"
-      with w_star show ?thesis by simp
-    next
-      assume "\<not>w = []"
-      with w_cases obtain a C where "w = [Tm a, Nt C]" by blast
-      with w_star show ?thesis
-        using derives_T_Cons[of P a "[Nt C]" "[Nt B]"] by simp
-    qed
-  qed simp
-qed
-
 lemma mult_derive_to_nxts:
   assumes "rlin2 P"
   shows "A\<in>M \<Longrightarrow> P \<turnstile> [Nt A] \<Rightarrow>* map Tm w @ [Nt B] \<Longrightarrow> B \<in> nxts_rlin2_set P M w"
@@ -250,30 +148,10 @@ next
     unfolding nxt_rlin2_set_def nxt_rlin2_def by auto
 qed
 
-lemma rlin2_tms_eps:
-  assumes "rlin2 P"
-      and "P \<turnstile> [Nt A] \<Rightarrow>* map Tm w"
-    shows "\<exists>B. P \<turnstile> [Nt A] \<Rightarrow>* map Tm w @ [Nt B] \<and> (B,[]) \<in> P"
-proof -
-  from assms(2) have "\<exists>v. P \<turnstile> [Nt A] \<Rightarrow>* v \<and> P \<turnstile> v \<Rightarrow> map Tm w"
-    using rtranclp.cases by force
-  then obtain v where v_star: "P \<turnstile> [Nt A] \<Rightarrow>* v" and v_step: "P \<turnstile> v \<Rightarrow> map Tm w" by blast
-  from v_step have "\<exists>u1 u2 C \<alpha>. v = u1 @ [Nt C] @ u2 \<and> map Tm w = u1 @ \<alpha> @ u2 \<and> (C,\<alpha>) \<in> P"
-    using derive.cases by fastforce
-  then obtain u1 u2 C \<alpha> where v_def: "v = u1 @ [Nt C] @ u2" and w_def: "map Tm w = u1 @ \<alpha> @ u2" and C_prod: "(C,\<alpha>) \<in> P" by blast
-  have "\<nexists>A. Nt A \<in> set (map Tm w)" by auto
-  with w_def have "\<nexists>A. Nt A \<in> set \<alpha>" 
-    by (metis Un_iff set_append)
-  then have "\<nexists>a A. \<alpha> = [Tm a, Nt A]" by auto
-  with assms(1) C_prod have alpha_eps: "\<alpha> = []"
-    using rlin2_def by force
-  from v_star assms(1) v_def have u2_eps: "u2 = []"
-    using rlin2_derive[of P "[Nt A]"] by simp
-  from w_def alpha_eps u2_eps have u1_def: "u1 = map Tm w" by simp
-  from v_star v_def u1_def u2_eps have 1: "P \<turnstile> [Nt A] \<Rightarrow>* map Tm w @ [Nt C]" by simp
-  from alpha_eps C_prod have 2: "(C,[]) \<in> P"  by simp
-  from 1 2 show ?thesis by auto
-qed
+text
+\<open>\<open>accepted P A w\<close> is defined as following and checks whether there exists a reachable non-terminal \<open>Z\<close> such that \<open>(Z,[])\<close> is in the
+ production set \<open>P\<close>. In the automata level this corresponds a reachable final state and therefore the name \<open>accepted\<close>. We show that
+ a word \<open>w\<close>, starting from the non-terminal \<open>A\<close>, is in the language of \<open>P\<close> if and only if \<open>accepted P A w\<close>\<close>
 
 definition "accepted P A w = (\<exists>Z \<in> nxts_rlin2_set P {A} w. (Z,[]) \<in> P)"
 
@@ -312,6 +190,5 @@ theorem Lang_iff_accepted_if_rlin2:
 assumes "rlin2 P"
 shows "w \<in> Lang P A \<longleftrightarrow> accepted P A w"
   using accepted_if_Lang[OF assms] Lang_if_accepted by fast
-
 
 end
