Taskin/UsingPumpingLemmaRe.thy
@@ -54,11 +54,18 @@ proof (rule ccontr)
   qed
 qed
 
+text
+\<open>Most of the time pumping lemma is used in the contrapositive form if it is used to prove that a production set cannot be right linear\<close>
+
 theorem pumping_lemma_re_contr:
   assumes "finite P"
       and "\<forall>n. \<exists>w \<in> Lang P A. length w \<ge> n \<and> (\<forall>x y z. w = x@y@z \<and> length y \<ge> 1 \<and> length (x@y) \<le> n \<longrightarrow> (\<exists>i. x@(y\<^sup>*i)@z \<notin> Lang P A))" 
     shows "\<not>rlin2 P"
 using assms pumping_lemma_re[of P A] by metis
+
+text
+\<open>The following theorem proves that the language \<open>a^nb^n\<close> cannot be produced by a right linear production set, using the contrapositive form 
+ of the pumping lemma\<close>
 
 theorem not_rlin2_ab:
   assumes "Lang P A = {([Tm a]\<^sup>*n)@([Tm b]\<^sup>*n)|n. n\<in>\<nat>}"
